Unique Maximum Element (#113)
* Unique minimum proof

* adding unique maximum and updating structure

* format

* format

* remove duplicates in dafny subfolder

* remove empty line

* space fix

* remove equivalence relation and symmetric

* format space

* comment style

* comments again

* refinement

* naming

* naming

* fix typos

* remove empty space

* remove line

* format

* newline

* format

src/dafny/Relations.dfy
@@ -75,9 +75,42 @@ module {:options "-functionSyntax:4"} Dafny.Relations {
     && Connected(R)
   }
 
+  ghost predicate PreOrdering<T(!new)>(R: (T, T) -> bool) {
+    && Reflexive(R)
+    && Transitive(R)
+  }
+
+  ghost predicate PartialOrdering<T(!new)>(R: (T, T) -> bool) {
+    && Reflexive(R)
+    && Transitive(R)
+    && AntiSymmetric(R)
+  }
+
   ghost predicate EquivalenceRelation<T(!new)>(R: (T, T) -> bool) {
     && Reflexive(R)
     && Symmetric(R)
     && Transitive(R)
+  }
+
+  /** An element in an ordered set is called a least element (or a minimum), if it is less than 
+      every other element of the set. */
+  ghost predicate IsLeast<T>(R: (T, T) -> bool, min: T, s: set<T>) {
+    min in s && forall x | x in s :: R(min, x)
+  }
+
+  /** An element in an ordered set is called a minimal element, if no other element is less than it. */
+  ghost predicate IsMinimal<T>(R: (T, T) -> bool, min: T, s: set<T>) {
+    min in s && forall x | x in s && R(x, min) :: R(min, x)
+  }
+
+  /** An element in an ordered set is called a greatest element (or a maximum), if it is greater than 
+      every other element of the set. */
+  ghost predicate IsGreatest<T>(R: (T, T) -> bool, max: T, s: set<T>) {
+    max in s && forall x | x in s :: R(x, max)
+  }
+
+  /** An element in an ordered set is called a maximal element, if no other element is greater than it. */
+  ghost predicate IsMaximal<T>(R: (T, T) -> bool, max: T, s: set<T>) {
+    max in s && forall x | x in s && R(max, x) :: R(x, max)
   }
 }
